Foundation/Modal/Kripke/Hilbert/KT.lean
@@ -5,15 +5,11 @@ namespace LO.Modal
 open Kripke
 open Geachean
 
-abbrev Kripke.ReflexiveFrameClass : FrameClass := { F | Reflexive F }
-
 namespace Hilbert.KT
 
 instance Kripke.sound : Sound (Hilbert.KT) (Kripke.ReflexiveFrameClass) := by
-  convert Hilbert.Geach.Kripke.sound (G := {⟨0, 0, 1, 0⟩});
-  . exact eq_Geach;
-  . unfold ReflexiveFrameClass MultiGeacheanConfluentFrameClass MultiGeachean;
-    simp [Geachean.reflexive_def];
+  have := FrameClass.definedBy_with_axiomK ReflexiveFrameClass.definedByAxiomT;
+  infer_instance
 
 instance Kripke.consistent : Entailment.Consistent (Hilbert.KT) := by
   convert Hilbert.Geach.Kripke.Consistent (G := {⟨0, 0, 1, 0⟩});
