Foundation/Modal/Logic/Sublogic.lean
@@ -556,6 +556,32 @@ theorem K4_ssubset_GL : Logic.K4 ⊂ Logic.GL := by
     . exact Hilbert.K4.unprovable_AxiomL;
 instance : ProperSublogic Logic.K4 Logic.GL := ⟨K4_ssubset_GL⟩
 
+instance : ProperSublogic Logic.K4 Logic.K4Dot1 := ⟨by
+  constructor;
+  . exact Hilbert.weakerThan_of_dominate_axioms (by simp) |>.subset;
+  . suffices ∃ φ, Hilbert.K4Dot1 ⊢! φ ∧ ¬TransitiveFrameClass ⊧ φ by simpa [K4.eq_TransitiveKripkeFrameClass_Logic];
+    use (Axioms.M (.atom 0));
+    constructor;
+    . exact axiomM!;
+    . apply Formula.Kripke.ValidOnFrameClass.not_of_exists_model_world;
+      use ⟨⟨Fin 1, λ x y => False⟩, λ w _ => False⟩, 0;
+      simp [Transitive, Semantics.Realize, Satisfies];
+⟩
+
+instance : ProperSublogic Logic.S4 Logic.S4Dot1 := ⟨by
+  constructor;
+  . exact Hilbert.weakerThan_of_dominate_axioms (by simp) |>.subset;
+  . suffices ∃ φ, Hilbert.S4Dot1 ⊢! φ ∧ ¬ReflexiveTransitiveFrameClass ⊧ φ by simpa [S4.eq_ReflexiveTransitiveKripkeFrameClass_Logic];
+    use (Axioms.M (.atom 0));
+    constructor;
+    . exact axiomM!;
+    . apply Formula.Kripke.ValidOnFrameClass.not_of_exists_model_world;
+      let M : Model := ⟨⟨Fin 2, λ x y => True⟩, λ w _ => w = 0⟩;
+      use M, 0;
+      suffices ∃ x, x ≠ (0 : M.World) by simpa [M, Transitive, Reflexive, Semantics.Realize, Satisfies];
+      use 1;
+      trivial;
+⟩
 
 theorem S4_ssubset_S4Dot2 : Logic.S4 ⊂ Logic.S4Dot2 := by
   constructor;
